NLustre/NLSyntax.v
@@ -186,30 +186,35 @@ Module Type NLSYNTAX
   (* XXX: computationally, the following [gather_*] are useless: they
      are only used to simplify the proofs. See [gather_eqs_fst_spec]
      and [gather_eqs_snd_spec]. *)
-  Definition gather_mem (eqs: list equation): idents :=
-    concatMap (fun eq => match eq with
-                      | EqDef _ _ _
-                      | EqApp _ _ _ _ _ => []
-                      | EqFby x _ _ _ => [x]
-                      end) eqs.
+  Definition gather_mem_eq (eq: equation): idents :=
+    match eq with
+    | EqDef _ _ _
+    | EqApp _ _ _ _ _ => []
+    | EqFby x _ _ _ => [x]
+    end.
 
-  Definition gather_insts (eqs: list equation): list (ident * ident) :=
-    concatMap (fun eq => match eq with
-                      | EqDef _ _ _
-                      | EqFby _ _ _ _ => []
-                      | EqApp i _ f _ _ =>
-                        match i with
-                        | [] => []
-                        | i :: _ => [(i,f)]
-                        end
-                      end) eqs.
+  Definition gather_inst_eq (eq: equation): list (ident * ident) :=
+    match eq with
+    | EqDef _ _ _
+    | EqFby _ _ _ _ => []
+    | EqApp i _ f _ _ =>
+      match i with
+      | [] => []
+      | i :: _ => [(i,f)]
+      end
+    end.
 
-  Definition gather_app_vars (eqs: list equation): idents :=
-    concatMap (fun eq => match eq with
-                      | EqDef _ _ _
-                      | EqFby _ _ _ _ => []
-                      | EqApp xs _ _ _ _ => tl xs
-                      end) eqs.
+  Definition gather_app_vars_eq (eq: equation): idents :=
+    match eq with
+    | EqDef _ _ _
+    | EqFby _ _ _ _ => []
+    | EqApp xs _ _ _ _ => tl xs
+    end.
+
+  Definition gather_mems := concatMap gather_mem_eq.
+  Definition gather_insts := concatMap gather_inst_eq.
+  Definition gather_app_vars := concatMap gather_app_vars_eq.
+
 End NLSYNTAX.
 
 Module NLSyntaxFun
